[pairing heaps] more refinement

Weidenbach_Book/IsaSAT/Pairing_Heaps_Impl.thy
@@ -45,13 +45,13 @@ fun hp_read_nxt' :: \<open>_\<close> where
   \<open>hp_read_nxt' i (\<V>, arr, h) = hp_read_nxt i arr\<close>
 
 lemma op_hp_read_nxt_imp_spec:
-  \<open>(xs, ys) \<in> \<langle>R,S\<rangle>pairing_heaps_rel \<Longrightarrow> j \<in> fst ys \<Longrightarrow> (i,j)\<in>nat_rel \<Longrightarrow>
+  \<open>(xs, ys) \<in> \<langle>R,S\<rangle>pairing_heaps_rel \<Longrightarrow> (i,j)\<in>nat_rel \<Longrightarrow> j \<in> fst ys \<Longrightarrow>
   (op_hp_read_nxt_imp i xs, hp_read_nxt' j ys) \<in> R\<close>
   unfolding op_hp_read_nxt_imp_def
   by (auto simp: pairing_heaps_rel_def map_fun_rel_def)
 
 lemma mop_hp_read_nxt_imp_spec:
-  \<open>(xs, ys) \<in> \<langle>R,S\<rangle>pairing_heaps_rel \<Longrightarrow> j \<in> fst ys \<Longrightarrow> (i,j)\<in>nat_rel \<Longrightarrow>
+  \<open>(xs, ys) \<in> \<langle>R,S\<rangle>pairing_heaps_rel \<Longrightarrow> (i,j)\<in>nat_rel \<Longrightarrow> j \<in> fst ys \<Longrightarrow>
   mop_hp_read_nxt_imp i xs \<le> SPEC (\<lambda>a. (a, hp_read_nxt' j ys) \<in> R)\<close>
   unfolding mop_hp_read_nxt_imp_def
   apply refine_vcg
@@ -76,13 +76,13 @@ fun hp_read_prev' :: \<open>_\<close> where
   \<open>hp_read_prev' i (\<V>, arr, h) = hp_read_prev i arr\<close>
 
 lemma op_hp_read_prev_imp_spec:
-  \<open>(xs, ys) \<in> \<langle>R,S\<rangle>pairing_heaps_rel \<Longrightarrow> j \<in> fst ys \<Longrightarrow> (i,j)\<in>nat_rel \<Longrightarrow>
+  \<open>(xs, ys) \<in> \<langle>R,S\<rangle>pairing_heaps_rel \<Longrightarrow> (i,j)\<in>nat_rel \<Longrightarrow> j \<in> fst ys \<Longrightarrow>
   (op_hp_read_prev_imp i xs, hp_read_prev' j ys) \<in> R\<close>
   unfolding op_hp_read_prev_imp_def
   by (auto simp: pairing_heaps_rel_def map_fun_rel_def)
 
 lemma mop_hp_read_prev_imp_spec:
-  \<open>(xs, ys) \<in> \<langle>R,S\<rangle>pairing_heaps_rel \<Longrightarrow> j \<in> fst ys \<Longrightarrow> (i,j)\<in>nat_rel \<Longrightarrow>
+  \<open>(xs, ys) \<in> \<langle>R,S\<rangle>pairing_heaps_rel \<Longrightarrow> (i,j)\<in>nat_rel \<Longrightarrow> j \<in> fst ys \<Longrightarrow>
   mop_hp_read_prev_imp i xs \<le> SPEC (\<lambda>a. (a, hp_read_prev' j ys) \<in> R)\<close>
   unfolding mop_hp_read_prev_imp_def
   apply refine_vcg
@@ -107,13 +107,13 @@ fun hp_read_child' :: \<open>_\<close> where
   \<open>hp_read_child' i (\<V>, arr, h) = hp_read_child i arr\<close>
 
 lemma op_hp_read_child_imp_spec:
-  \<open>(xs, ys) \<in> \<langle>R,S\<rangle>pairing_heaps_rel \<Longrightarrow> j \<in> fst ys \<Longrightarrow> (i,j)\<in>nat_rel \<Longrightarrow>
+  \<open>(xs, ys) \<in> \<langle>R,S\<rangle>pairing_heaps_rel \<Longrightarrow> (i,j)\<in>nat_rel \<Longrightarrow> j \<in> fst ys \<Longrightarrow>
   (op_hp_read_child_imp i xs, hp_read_child' j ys) \<in> R\<close>
   unfolding op_hp_read_child_imp_def
   by (auto simp: pairing_heaps_rel_def map_fun_rel_def)
 
 lemma mop_hp_read_child_imp_spec:
-  \<open>(xs, ys) \<in> \<langle>R,S\<rangle>pairing_heaps_rel \<Longrightarrow> j \<in> fst ys \<Longrightarrow> (i,j)\<in>nat_rel \<Longrightarrow>
+  \<open>(xs, ys) \<in> \<langle>R,S\<rangle>pairing_heaps_rel \<Longrightarrow> (i,j)\<in>nat_rel  \<Longrightarrow> j \<in> fst ys \<Longrightarrow>
   mop_hp_read_child_imp i xs \<le> SPEC (\<lambda>a. (a, hp_read_child' j ys) \<in> R)\<close>
   unfolding mop_hp_read_child_imp_def
   apply refine_vcg
@@ -137,13 +137,13 @@ fun hp_read_parent' :: \<open>_\<close> where
   \<open>hp_read_parent' i (\<V>, arr, h) = hp_read_parent i arr\<close>
 
 lemma op_hp_read_parent_imp_spec:
-  \<open>(xs, ys) \<in> \<langle>R,S\<rangle>pairing_heaps_rel \<Longrightarrow> j \<in> fst ys \<Longrightarrow> (i,j)\<in>nat_rel \<Longrightarrow>
+  \<open>(xs, ys) \<in> \<langle>R,S\<rangle>pairing_heaps_rel \<Longrightarrow> (i,j)\<in>nat_rel \<Longrightarrow> j \<in> fst ys \<Longrightarrow>
   (op_hp_read_parent_imp i xs, hp_read_parent' j ys) \<in> R\<close>
   unfolding op_hp_read_parent_imp_def
   by (auto simp: pairing_heaps_rel_def map_fun_rel_def)
  
 lemma mop_hp_read_parent_imp_spec:
-  \<open>(xs, ys) \<in> \<langle>R,S\<rangle>pairing_heaps_rel \<Longrightarrow> j \<in> fst ys \<Longrightarrow> (i,j)\<in>nat_rel \<Longrightarrow>
+  \<open>(xs, ys) \<in> \<langle>R,S\<rangle>pairing_heaps_rel \<Longrightarrow> (i,j)\<in>nat_rel \<Longrightarrow> j \<in> fst ys \<Longrightarrow>
   mop_hp_read_parent_imp i xs \<le> SPEC (\<lambda>a. (a, hp_read_parent' j ys) \<in> R)\<close>
   unfolding mop_hp_read_parent_imp_def
   apply refine_vcg
@@ -168,7 +168,7 @@ fun hp_read_score' :: \<open>_\<close> where
   \<open>hp_read_score' i (\<V>, arr, h) = (hp_read_score i arr)\<close>
 
 lemma mop_hp_read_score_imp_spec:
-  \<open>(xs, ys) \<in> \<langle>R,S\<rangle>pairing_heaps_rel \<Longrightarrow> j \<in> fst ys \<Longrightarrow> (i,j)\<in>nat_rel \<Longrightarrow>
+  \<open>(xs, ys) \<in> \<langle>R,S\<rangle>pairing_heaps_rel \<Longrightarrow> (i,j)\<in>nat_rel \<Longrightarrow> j \<in> fst ys \<Longrightarrow>
   mop_hp_read_score_imp i xs \<le> SPEC (\<lambda>a. (Some a, hp_read_score' j ys) \<in> S)\<close>
   unfolding mop_hp_read_score_imp_def
   apply refine_vcg
@@ -189,8 +189,8 @@ definition mop_hp_set_all_imp :: \<open>nat \<Rightarrow> _ \<Rightarrow> _ \<Ri
 
 
 lemma mop_hp_set_all_imp_spec:
-  \<open>(xs, ys) \<in> \<langle>R,S\<rangle>pairing_heaps_rel \<Longrightarrow> j \<in> fst ys \<Longrightarrow> (i,j)\<in>nat_rel \<Longrightarrow>
-   (p',p)\<in>R \<Longrightarrow> (q',q)\<in>R\<Longrightarrow>(r',r)\<in>R \<Longrightarrow> (s',s)\<in>R\<Longrightarrow> (Some t',t)\<in>S \<Longrightarrow>
+  \<open>(xs, ys) \<in> \<langle>R,S\<rangle>pairing_heaps_rel \<Longrightarrow>(i,j)\<in>nat_rel \<Longrightarrow>
+   (p',p)\<in>R \<Longrightarrow> (q',q)\<in>R\<Longrightarrow>(r',r)\<in>R \<Longrightarrow> (s',s)\<in>R\<Longrightarrow> (Some t',t)\<in>S \<Longrightarrow> j \<in> fst ys \<Longrightarrow> 
   mop_hp_set_all_imp i p' q' r' s' t' xs \<le> SPEC (\<lambda>a. (a, hp_set_all' j p q r s t ys) \<in> \<langle>R,S\<rangle>pairing_heaps_rel)\<close>
   unfolding mop_hp_set_all_imp_def
   apply refine_vcg
@@ -229,6 +229,9 @@ lemma source_node_spec:
   \<open>(xs, ys) \<in> \<langle>R,S\<rangle>pairing_heaps_rel \<Longrightarrow>
   (source_node_impl xs, source_node ys) \<in> R›
   by (auto simp: pairing_heaps_rel_def map_fun_rel_def)
+
+fun hp_update_child' where
+  \<open>hp_update_child' i p(\<V>, u, h) = (\<V>, hp_update_child i p u, h)\<close>
 
 fun hp_update_parents' where
   \<open>hp_update_parents' i p(\<V>, u, h) = (\<V>, hp_update_parents i p u, h)\<close>
@@ -335,7 +338,7 @@ lemma mop_hp_update_parent'_imp_spec:
 
 definition mop_hp_update_nxt'_imp :: \<open>nat \<Rightarrow> 'a option \<Rightarrow> ('a,'b)pairing_heaps_imp \<Rightarrow> ('a,'b)pairing_heaps_imp nres\<close> where
   \<open>mop_hp_update_nxt'_imp = (\<lambda>i v (prevs, nxts, parents, children). do {
-    ASSERT (i < length prevs);
+    ASSERT (i < length nxts);
     RETURN (prevs, nxts[i:=v], parents, children)
   })\<close>
 
@@ -354,9 +357,9 @@ lemma mop_hp_update_nxt'_imp_spec:
 
 
 definition mop_hp_update_child'_imp :: \<open>nat \<Rightarrow> 'a option \<Rightarrow> ('a,'b)pairing_heaps_imp \<Rightarrow> ('a,'b)pairing_heaps_imp nres\<close> where
-  \<open>mop_hp_update_child'_imp = (\<lambda>i v (prevs, childs, parents, children). do {
-    ASSERT (i < length prevs);
-    RETURN (prevs, childs[i:=v], parents, children)
+  \<open>mop_hp_update_child'_imp = (\<lambda>i v (prevs, nxts, children, parents, scores). do {
+    ASSERT (i < length children);
+    RETURN (prevs, nxts, children[i:=v], parents, scores)
   })\<close>
 
 
@@ -369,7 +372,7 @@ lemma mop_hp_update_child'_imp_spec:
   subgoal
     by (auto simp: pairing_heaps_rel_def map_fun_rel_def hp_update_prev_def)
   subgoal
-    by (force simp: pairing_heaps_rel_def map_fun_rel_def hp_update_child_def)
+    by (force simp add: pairing_heaps_rel_def map_fun_rel_def hp_update_child_def)
   done
 
 (*TODO it is kind of unclear whether we should use nat or have a conversion 'a \<Rightarrow> nat as locale*)
@@ -455,10 +458,10 @@ proof -
       using op_hp_read_parent_imp_spec[of xs ys \<open>\<langle>nat_rel\<rangle>option_rel\<close> \<open>\<langle>nat_rel\<rangle>option_rel\<close> \<open>the (source_node ys)\<close> \<open>the (source_node_impl xs)\<close>]
         source_node_spec[of xs ys  \<open>\<langle>nat_rel\<rangle>option_rel\<close> \<open>\<langle>nat_rel\<rangle>option_rel\<close>]
       by auto
+    subgoal by auto
     subgoal
       using source_node_spec[of xs ys  \<open>\<langle>nat_rel\<rangle>option_rel\<close> \<open>\<langle>nat_rel\<rangle>option_rel\<close>]
       by auto
-    subgoal by auto
     subgoal
       using source_node_spec[of xs ys  \<open>\<langle>nat_rel\<rangle>option_rel\<close> \<open>\<langle>nat_rel\<rangle>option_rel\<close>]
       by auto
@@ -472,8 +475,8 @@ proof -
     subgoal by auto
     subgoal using source_node_spec[of xs ys  \<open>\<langle>nat_rel\<rangle>option_rel\<close> \<open>\<langle>nat_rel\<rangle>option_rel\<close>] by auto
     subgoal by (auto intro!: update_source_node_impl_spec)
-    subgoal by auto
     subgoal using source_node_spec[of xs ys  \<open>\<langle>nat_rel\<rangle>option_rel\<close> \<open>\<langle>nat_rel\<rangle>option_rel\<close>] by auto
+    subgoal by auto
     subgoal by auto
     subgoal by auto
     subgoal by auto
@@ -536,6 +539,8 @@ lemma hp_link_alt_def:
     ASSERT (i \<noteq> j);
     ASSERT (i \<in> fst arr);
     ASSERT (j \<in> fst arr);
+    ASSERT (hp_read_score' i arr \<noteq> None);
+    ASSERT (hp_read_score' j arr \<noteq> None);
     let x = (the (hp_read_score' i arr)::'b::order);
     let y = (the (hp_read_score' j arr)::'b);
     let prev = hp_read_prev' i arr;
@@ -587,11 +592,15 @@ proof -
     subgoal by auto
     subgoal by auto
     subgoal by auto
+    subgoal by auto
+    subgoal by auto
     subgoal by simp (metis option.simps(2))
     done
   moreover have \<open>?B i j arr \<le> \<Down>Id (?A i j arr)\<close> for i j arr
     unfolding hp_link_def case_prod_beta f_def[symmetric]
     apply refine_vcg
+    subgoal by auto
+    subgoal by auto
     subgoal by auto
     subgoal by auto
     subgoal by auto
@@ -617,6 +626,67 @@ proof -
     done
 qed
 
+
+definition maybe_hp_update_prev' where
+  \<open>maybe_hp_update_prev' child ch arr =
+     (if child = None then arr else hp_update_prev' (the child) ch arr)\<close>
+
+definition maybe_hp_update_nxt' where
+  \<open>maybe_hp_update_nxt' child ch arr =
+     (if child = None then arr else hp_update_nxt' (the child) ch arr)\<close>
+
+definition maybe_hp_update_parents' where
+  \<open>maybe_hp_update_parents' child ch arr =
+     (if child = None then arr else hp_update_parents' (the child) ch arr)\<close>
+
+definition maybe_mop_hp_update_prev'_imp where
+  \<open>maybe_mop_hp_update_prev'_imp child ch arr =
+     (if child = None then RETURN arr else mop_hp_update_prev'_imp (the child) ch arr)\<close>
+
+definition maybe_mop_hp_update_nxt'_imp where
+  \<open>maybe_mop_hp_update_nxt'_imp child ch arr =
+     (if child = None then RETURN arr else mop_hp_update_nxt'_imp (the child) ch arr)\<close>
+
+definition maybe_mop_hp_update_child'_imp where
+  \<open>maybe_mop_hp_update_child'_imp child ch arr =
+     (if child = None then RETURN arr else mop_hp_update_child'_imp (the child) ch arr)\<close>
+
+definition maybe_mop_hp_update_parent'_imp where
+  \<open>maybe_mop_hp_update_parent'_imp child ch arr =
+     (if child = None then RETURN arr else mop_hp_update_parent'_imp (the child) ch arr)\<close>
+
+definition maybe_hp_update_child' where
+  \<open>maybe_hp_update_child' child ch arr =
+     (if child = None then arr else hp_update_child' (the child) ch arr)\<close>
+
+lemma maybe_mop_hp_update_prev'_imp_spec:
+  \<open>(xs, ys) \<in> \<langle>R,S\<rangle>pairing_heaps_rel \<Longrightarrow> (i,j)\<in>\<langle>nat_rel\<rangle>option_rel \<Longrightarrow> (j \<noteq> None \<Longrightarrow> the j \<in> fst ys) \<Longrightarrow>
+   (p',p)\<in>R \<Longrightarrow>
+  maybe_mop_hp_update_prev'_imp i p' xs \<le> SPEC (\<lambda>a. (a, maybe_hp_update_prev' j p ys) \<in> \<langle>R,S\<rangle>pairing_heaps_rel)\<close>
+  unfolding maybe_mop_hp_update_prev'_imp_def maybe_hp_update_prev'_def
+  by (refine_vcg mop_hp_update_prev'_imp_spec) auto
+
+lemma maybe_mop_hp_update_nxt'_imp_spec:
+  \<open>(xs, ys) \<in> \<langle>R,S\<rangle>pairing_heaps_rel \<Longrightarrow> (i,j)\<in>\<langle>nat_rel\<rangle>option_rel \<Longrightarrow> (j \<noteq> None \<Longrightarrow> the j \<in> fst ys) \<Longrightarrow> 
+   (p',p)\<in>R \<Longrightarrow>
+  maybe_mop_hp_update_nxt'_imp i p' xs \<le> SPEC (\<lambda>a. (a, maybe_hp_update_nxt' j p ys) \<in> \<langle>R,S\<rangle>pairing_heaps_rel)\<close>
+  unfolding maybe_mop_hp_update_nxt'_imp_def maybe_hp_update_nxt'_def
+  by (refine_vcg mop_hp_update_nxt'_imp_spec) auto
+
+lemma maybe_mop_hp_update_parent'_imp_spec:
+  \<open>(xs, ys) \<in> \<langle>R,S\<rangle>pairing_heaps_rel \<Longrightarrow> (i,j)\<in>\<langle>nat_rel\<rangle>option_rel \<Longrightarrow> (j \<noteq> None \<Longrightarrow> the j \<in> fst ys) \<Longrightarrow>
+   (p',p)\<in>R \<Longrightarrow>
+  maybe_mop_hp_update_parent'_imp i p' xs \<le> SPEC (\<lambda>a. (a, maybe_hp_update_parents' j p ys) \<in> \<langle>R,S\<rangle>pairing_heaps_rel)\<close>
+  unfolding maybe_mop_hp_update_parent'_imp_def maybe_hp_update_parents'_def
+  by (refine_vcg mop_hp_update_parent'_imp_spec) auto
+
+lemma maybe_mop_hp_update_child'_imp_spec:
+  \<open>(xs, ys) \<in> \<langle>R,S\<rangle>pairing_heaps_rel \<Longrightarrow> (i,j)\<in>\<langle>nat_rel\<rangle>option_rel \<Longrightarrow> (j \<noteq> None \<Longrightarrow> the j \<in> fst ys) \<Longrightarrow> 
+   (p',p)\<in>R \<Longrightarrow>
+  maybe_mop_hp_update_child'_imp i p' xs \<le> SPEC (\<lambda>a. (a, maybe_hp_update_child' j p ys) \<in> \<langle>R,S\<rangle>pairing_heaps_rel)\<close>
+  unfolding maybe_mop_hp_update_child'_imp_def maybe_hp_update_child'_def
+  by (refine_vcg mop_hp_update_child'_imp_spec) auto
+
 definition mop_hp_link_imp  :: \<open>nat \<Rightarrow>nat \<Rightarrow>(nat, 'b::ord)pairing_heaps_imp \<Rightarrow> _ nres\<close> where
    \<open>mop_hp_link_imp = (\<lambda>i j arr. do {
     ASSERT (i \<noteq> j);
@@ -636,16 +706,33 @@ definition mop_hp_link_imp  :: \<open>nat \<Rightarrow>nat \<Rightarrow>(nat, 'b
     RETURN (arr, parent)
       })\<close>
 
-(*TODO: this is too annoying to refine: make a maybe_mop_hp_update_parent'_imp to avoid the annoying case splitting*)
 
+lemma fst_hp_update_simp[simp]:
+  \<open>fst (hp_update_prev' i x arr) = fst arr›
+  \<open>fst (hp_update_nxt' i x arr) = fst arr›
+  \<open>fst (hp_update_child' i x arr) = fst arr›
+  \<open>fst (hp_update_parents' i x arr) = fst arr›
+  by (solves \<open>cases arr; auto\<close>)+
 
-lemma mop_hp_insert_impl_spec:
+lemma fst_maybe_hp_update_simp[simp]:
+  \<open>fst (maybe_hp_update_prev' i y arr) = fst arr›
+  \<open>fst (maybe_hp_update_nxt' i y arr) = fst arr›
+  \<open>fst (maybe_hp_update_child' i y arr) = fst arr›
+  \<open>fst (maybe_hp_update_parents' i y arr) = fst arr›
+  by (solves \<open>cases arr; cases i; auto simp: maybe_hp_update_prev'_def maybe_hp_update_nxt'_def
+    maybe_hp_update_child'_def maybe_hp_update_parents'_def\<close>)+
+
+lemma mop_hp_link_imp_spec:
   assumes \<open>(xs, ys) \<in> \<langle>\<langle>nat_rel\<rangle>option_rel,\<langle>nat_rel\<rangle>option_rel\<rangle>pairing_heaps_rel\<close> \<open>(i,j)\<in>nat_rel\<close> \<open>(w,w')\<in>nat_rel\<close>
   shows \<open>mop_hp_link_imp i w xs \<le> \<Down>(\<langle>\<langle>nat_rel\<rangle>option_rel,\<langle>nat_rel\<rangle>option_rel\<rangle>pairing_heaps_rel \<times>\<^sub>r nat_rel) (hp_link j w' ys)\<close>
 proof -
   have [refine]: \<open>(Some i, Some j) \<in> \<langle>nat_rel\<rangle>option_rel\<close>
     using assms by auto
-  define f where \<open>f i j x y \<equiv> (if y < x then (i::nat, j::nat, x::nat, y::nat) else (j, i, y, x))\<close> for i j x y
+  define f where \<open>f i j x y \<equiv> RETURN (if y < x then (i::nat, j::nat, x::nat, y::nat) else (j, i, y, x))\<close> for i j x y
+  have Hf: \<open>do {let (parent, ch, w\<^sub>p, w\<^sub>c\<^sub>h) = (if y < x then (i, j, x, y) else (j, i, y, x)); P parent ch w\<^sub>p w\<^sub>c\<^sub>h} =
+    do {(parent, ch, w\<^sub>p, w\<^sub>c\<^sub>h) \<leftarrow> f i j x y; P parent ch w\<^sub>p w\<^sub>c\<^sub>h}\<close> for i j x y w xs P
+    unfolding f_def let_to_bind_conv ..
+
   have K: \<open>hp_read_child' (the (source_node ys)) ys \<noteq> None \<longrightarrow>
     the (hp_read_child' (the (source_node ys)) ys) \<in> \<V> \<Longrightarrow> the (source_node ys) \<in> fst ys \<Longrightarrow>
     op_hp_read_child_imp (the (source_node_impl xs)) xs \<noteq> None \<Longrightarrow>
@@ -653,19 +740,33 @@ proof -
     using op_hp_read_child_imp_spec[of xs ys \<open>\<langle>nat_rel\<rangle>option_rel\<close> \<open>\<langle>nat_rel\<rangle>option_rel\<close> \<open>the (source_node ys)\<close> \<open>the (source_node_impl xs)\<close>]
       source_node_spec[of xs ys  \<open>\<langle>nat_rel\<rangle>option_rel\<close> \<open>\<langle>nat_rel\<rangle>option_rel\<close>] assms
     by auto
+  have [refine]: \<open>(x,x')\<in>nat_rel \<Longrightarrow> (y,y')\<in>nat_rel\<Longrightarrow>
+    f i w x y \<le> \<Down> (nat_rel \<times>\<^sub>r nat_rel \<times>\<^sub>r nat_rel \<times>\<^sub>r nat_rel) (f j w' x' y')\<close> for x' y' x y
+   using assms by auto
   show ?thesis
     using assms
-      op_hp_read_nxt_imp_spec[OF assms(1) _ assms(2)]
-      op_hp_read_prev_imp_spec[OF assms(1) _ assms(2)]
-      op_hp_read_child_imp_spec[OF assms(1) _ assms(2)]
-      op_hp_read_nxt_imp_spec[OF assms(1) _ assms(3)]
-    unfolding mop_hp_link_imp_def hp_link_alt_def f_def[symmetric]
+      op_hp_read_nxt_imp_spec[OF assms(1) assms(2)]
+      op_hp_read_prev_imp_spec[OF assms(1) assms(2)]
+      op_hp_read_child_imp_spec[OF assms(1) assms(2)]
+      op_hp_read_nxt_imp_spec[OF assms(1) assms(3)]
+    unfolding mop_hp_link_imp_def hp_link_alt_def Hf
+      maybe_mop_hp_update_parent'_imp_def[symmetric]
+      maybe_mop_hp_update_prev'_imp_def[symmetric]
+      maybe_mop_hp_update_nxt'_imp_def[symmetric]
+      maybe_hp_update_prev'_def[symmetric]
+      maybe_hp_update_parents'_def[symmetric]
+      maybe_hp_update_nxt'_def[symmetric]
+    apply -
     apply (refine_vcg mop_hp_set_all_imp_spec[where R=\<open>\<langle>nat_rel\<rangle>option_rel\<close> and S=\<open>\<langle>nat_rel\<rangle>option_rel\<close>]
       mop_hp_read_score_imp_spec[where R=\<open>\<langle>nat_rel\<rangle>option_rel\<close> and S=\<open>\<langle>nat_rel\<rangle>option_rel\<close> and ys=ys and i=i and j=j]
       mop_hp_read_score_imp_spec[where R=\<open>\<langle>nat_rel\<rangle>option_rel\<close> and S=\<open>\<langle>nat_rel\<rangle>option_rel\<close> and ys=ys and i=w and j=w']
       Some_x_y_option_theD[where S=nat_rel]
       mop_hp_update_parent'_imp_spec[where R=\<open>\<langle>nat_rel\<rangle>option_rel\<close> and S=\<open>\<langle>nat_rel\<rangle>option_rel\<close>]
-      mop_hp_update_prev'_imp_spec[where R=\<open>\<langle>nat_rel\<rangle>option_rel\<close> and S=\<open>\<langle>nat_rel\<rangle>option_rel\<close> and j=\<open>the (hp_read_child' (the (source_node ys)) ys)\<close>])
+      mop_hp_update_prev'_imp_spec[where R=\<open>\<langle>nat_rel\<rangle>option_rel\<close> and S=\<open>\<langle>nat_rel\<rangle>option_rel\<close> and j=\<open>the (hp_read_child' (the (source_node ys)) ys)\<close>]
+      maybe_mop_hp_update_parent'_imp_spec[where R=\<open>\<langle>nat_rel\<rangle>option_rel\<close> and S=\<open>\<langle>nat_rel\<rangle>option_rel\<close>]
+      maybe_mop_hp_update_prev'_imp_spec[where R=\<open>\<langle>nat_rel\<rangle>option_rel\<close> and S=\<open>\<langle>nat_rel\<rangle>option_rel\<close>]
+      maybe_mop_hp_update_nxt'_imp_spec[where R=\<open>\<langle>nat_rel\<rangle>option_rel\<close> and S=\<open>\<langle>nat_rel\<rangle>option_rel\<close>]
+      op_hp_read_child_imp_spec[where R=\<open>\<langle>nat_rel\<rangle>option_rel\<close> and S=\<open>\<langle>nat_rel\<rangle>option_rel\<close>])
     subgoal by (auto dest: source_node_spec)
     subgoal by auto
     subgoal by auto
@@ -676,11 +777,27 @@ proof -
     subgoal by auto
     subgoal by auto
     subgoal by auto
-    subgoal by (rule op_hp_read_child_imp_spec) (auto intro!: op_hp_read_child_imp_spec)
-    subgoal by (rule op_hp_read_child_imp_spec) (auto intro!: op_hp_read_child_imp_spec)
     subgoal by auto
     subgoal by auto
-    oops
+    subgoal by auto
+    subgoal by auto
+    subgoal by auto
+    subgoal by auto
+    apply (solves auto)
+    subgoal by auto
+    subgoal by auto
+    apply (solves auto)
+    subgoal by simp
+    apply (solves auto)
+    apply (solves auto)
+    subgoal by simp
+    apply (solves auto)
+    subgoal by auto
+    subgoal by auto
+    subgoal by auto
+    subgoal by auto
+    done
+qed
 
 lemma vsids_pass\<^sub>1_alt_def:
   \<open>vsids_pass\<^sub>1 = (\<lambda>(arr::'a set \<times> ('a,'c::order) hp_fun \<times> 'a option) (j::'a). do {
@@ -730,9 +847,7 @@ proof -
     done
 qed
 
-term vsids_pass\<^sub>1
-
-definition mop_vsids_pass\<^sub>1_imp :: \<open>(nat, 'b)pairing_heaps_imp \<Rightarrow> nat \<Rightarrow> _ nres\<close> where
+definition mop_vsids_pass\<^sub>1_imp :: \<open>(nat, 'b::ord)pairing_heaps_imp \<Rightarrow> nat \<Rightarrow> _ nres\<close> where
   \<open>mop_vsids_pass\<^sub>1_imp = (\<lambda>arr j. do {
   (arr, j, n) \<leftarrow> WHILE\<^sub>T(\<lambda>(arr, j, _). j \<noteq> None)
   (\<lambda>(arr, j, n). do {
@@ -753,19 +868,216 @@ definition mop_vsids_pass\<^sub>1_imp :: \<open>(nat, 'b)pairing_heaps_imp \<Rig
  })\<close>
 
 
-lemma mop_hp_insert_impl_spec:
+lemma mop_vsids_pass\<^sub>1_imp_spec:
   assumes \<open>(xs, ys) \<in> \<langle>\<langle>nat_rel\<rangle>option_rel,\<langle>nat_rel\<rangle>option_rel\<rangle>pairing_heaps_rel\<close> \<open>(i,j)\<in>nat_rel\<close>
-  shows \<open>mop_vsids_pass\<^sub>1_imp xs i \<le> \<Down>(\<langle>\<langle>nat_rel\<rangle>option_rel,\<langle>nat_rel\<rangle>option_rel\<rangle>pairing_heaps_rel) (vsids_pass\<^sub>1 ys j)\<close>
+  shows \<open>mop_vsids_pass\<^sub>1_imp xs i \<le> \<Down>(\<langle>\<langle>nat_rel\<rangle>option_rel,\<langle>nat_rel\<rangle>option_rel\<rangle>pairing_heaps_rel \<times>\<^sub>r nat_rel) (vsids_pass\<^sub>1 ys j)\<close>
 proof -
-  let ?R = \<open>{((arr, j, n), ((arr', j', _, n'))). (arr, arr') \<in> \<langle>\<langle>nat_rel\<rangle>option_rel,\<langle>nat_rel\<rangle>option_rel\<rangle>pairing_heaps_rel \<and>
-     (j, j') \<in> \<langle>nat_rel\<rangle>option_rel \<and> (n,n')\<in>Id}\<close>
+  let ?R = \<open>{((arr, j, n), (arr', j', _, n')). (arr, arr') \<in> \<langle>\<langle>nat_rel\<rangle>option_rel,\<langle>nat_rel\<rangle>option_rel\<rangle>pairing_heaps_rel \<and>
+    (j, j') \<in> \<langle>nat_rel\<rangle>option_rel \<and> (n,n')\<in>Id}\<close>
+  have K[refine0]: \<open>((xs, Some i, i), ys, Some j, 0, j) \<in> ?R\<close>
+    using assms by auto
   show ?thesis
     unfolding mop_vsids_pass\<^sub>1_imp_def vsids_pass\<^sub>1_alt_def
-    apply (refine_vcg mop_hp_insert_impl_spec WHILET_refine[where ?R=R])
-    subgoal
-    oops
+    apply (refine_vcg mop_hp_insert_impl_spec WHILET_refine[where R= ?R]
+      mop_hp_read_nxt_imp_spec[where R=\<open>\<langle>nat_rel\<rangle>option_rel\<close> and S=\<open>\<langle>nat_rel\<rangle>option_rel\<close>]
+      mop_hp_link_imp_spec)
+    subgoal by auto
+    subgoal by auto
+    subgoal by auto
+    subgoal by auto
+    subgoal by auto
+    subgoal by auto
+    subgoal by auto
+    subgoal by auto
+    subgoal by auto
+    subgoal by auto
+    subgoal by auto
+    subgoal by auto
+    subgoal by auto
+    subgoal by auto
+    done
+qed
 
-(*TODO next:*)
-  term vsids_pass\<^sub>1
-      term vsids_pass\<^sub>2
+lemma vsids_pass\<^sub>2_alt_def:
+  \<open>vsids_pass\<^sub>2 = (\<lambda>arr (j::'a). do {
+  ASSERT (j \<in> fst arr);
+  let nxt = hp_read_prev' j arr;
+  (arr, j, leader, _) \<leftarrow> WHILE\<^sub>T(\<lambda>(arr, j, leader, e). j \<noteq> None)
+  (\<lambda>(arr, j, leader, e::nat). do {
+    if j = None then RETURN (arr, None, leader, e)
+    else do {
+      let j = the j;
+      ASSERT (j \<in> fst arr);
+      let nnxt = hp_read_prev' j arr;
+      (arr, n) \<leftarrow> hp_link j leader arr;
+      RETURN (arr, nnxt, n, e+1)
+   }
+  })
+  (arr, nxt, j, 1::nat);
+  RETURN (update_source_node (Some leader) arr)
+  })\<close> (is \<open>?A = ?B\<close>)
+proof -
+  have K[refine]: \<open>(((fst i, fst (snd i), snd (snd i)), hp_read_prev arr (fst (snd i)), arr, 1::nat), i,
+  hp_read_prev' arr i, arr, 1::nat)
+    \<in> Id \<times>\<^sub>r \<langle>Id\<rangle>option_rel \<times>\<^sub>r Id \<times>\<^sub>r Id\<close>
+    \<open>((i, hp_read_prev' arr i, arr, 1), (fst i, fst (snd i), snd (snd i)),
+  hp_read_prev arr (fst (snd i)), arr, 1) \<in> Id \<times>\<^sub>r \<langle>Id\<rangle>option_rel \<times>\<^sub>r Id \<times>\<^sub>r Id\<close>
+    for i arr
+    by auto
+  have [refine]: \<open>(a,a')\<in>Id \<Longrightarrow> (b,b')\<in>Id \<Longrightarrow> (c,c')\<in>Id \<Longrightarrow> hp_link a b c \<le>\<Down>Id (hp_link a' b' c')\<close> for a b c a' b' c'
+    by auto
+  have \<open>?A i arr \<le> \<Down>Id (?B i arr)\<close> for i arr
+    unfolding vsids_pass\<^sub>2_def case_prod_beta[of _ i] case_prod_beta[of _ \<open>snd i\<close>]
+    by refine_vcg (solves auto)+
+  moreover have \<open>?B i arr \<le> \<Down>Id (?A i arr)\<close> for i arr
+    unfolding vsids_pass\<^sub>2_def case_prod_beta[of _ i] case_prod_beta[of _ \<open>snd i\<close>]
+    by refine_vcg (solves \<open>auto intro!: ext bind_cong[OF refl] simp: Let_def\<close>)+
+  ultimately show ?thesis unfolding Down_id_eq apply -
+    apply (intro ext)
+    apply (rule antisym)
+    apply assumption+
+    done
+qed
+
+definition mop_vsids_pass\<^sub>2_imp where
+  \<open>mop_vsids_pass\<^sub>2_imp = (\<lambda>arr (j::nat). do {
+  nxt \<leftarrow> mop_hp_read_prev_imp j arr;
+  (arr, j, leader) \<leftarrow> WHILE\<^sub>T(\<lambda>(arr, j, leader). j \<noteq> None)
+  (\<lambda>(arr, j, leader). do {
+    if j = None then RETURN (arr, None, leader)
+    else do {
+      let j = the j;
+      nnxt \<leftarrow> mop_hp_read_prev_imp j arr;
+      (arr, n) \<leftarrow> mop_hp_link_imp j leader arr;
+      RETURN (arr, nnxt, n)
+   }
+  })
+  (arr, nxt, j);
+  RETURN (update_source_node_impl (Some leader) arr)
+  })\<close>
+
+lemma mop_vsids_pass\<^sub>2_imp_spec:
+  assumes \<open>(xs, ys) \<in> \<langle>\<langle>nat_rel\<rangle>option_rel,\<langle>nat_rel\<rangle>option_rel\<rangle>pairing_heaps_rel\<close> \<open>(i,j)\<in>nat_rel\<close>
+  shows \<open>mop_vsids_pass\<^sub>2_imp xs i \<le> \<Down>(\<langle>\<langle>nat_rel\<rangle>option_rel,\<langle>nat_rel\<rangle>option_rel\<rangle>pairing_heaps_rel) (vsids_pass\<^sub>2 ys j)\<close>
+proof -
+  let ?R = \<open>{((arr, j, n), (arr', j', n', _)). (arr, arr') \<in> \<langle>\<langle>nat_rel\<rangle>option_rel,\<langle>nat_rel\<rangle>option_rel\<rangle>pairing_heaps_rel \<and>
+    (j, j') \<in> \<langle>nat_rel\<rangle>option_rel \<and> (n,n')\<in>Id}\<close>
+  have K[refine0]: \<open>((xs, Some i, i), ys, Some j, j, 0) \<in> ?R\<close>
+    using assms by auto
+  show ?thesis
+    using assms
+    unfolding mop_vsids_pass\<^sub>2_imp_def vsids_pass\<^sub>2_alt_def
+    apply (refine_vcg mop_hp_insert_impl_spec WHILET_refine[where R= ?R]
+      mop_hp_read_nxt_imp_spec[where R=\<open>\<langle>nat_rel\<rangle>option_rel\<close> and S=\<open>\<langle>nat_rel\<rangle>option_rel\<close>]
+      mop_hp_read_prev_imp_spec[where R=\<open>\<langle>nat_rel\<rangle>option_rel\<close> and S=\<open>\<langle>nat_rel\<rangle>option_rel\<close>]
+      mop_hp_link_imp_spec mop_vsids_pass\<^sub>1_imp_spec
+      update_source_node_impl_spec)
+    subgoal by auto
+    subgoal by auto
+    subgoal by auto
+    subgoal by auto
+    subgoal by auto
+    subgoal by auto
+    subgoal by auto
+    subgoal by auto
+    subgoal by auto
+    subgoal by auto
+    subgoal by auto
+    subgoal by auto
+    done
+qed
+
+definition mop_merge_pairs_imp where
+  \<open>mop_merge_pairs_imp arr j = do {
+    (arr, j) \<leftarrow> mop_vsids_pass\<^sub>1_imp arr j;
+    mop_vsids_pass\<^sub>2_imp arr j
+  }\<close>
+
+
+lemma mop_merge_pairs_imp_spec:
+  assumes \<open>(xs, ys) \<in> \<langle>\<langle>nat_rel\<rangle>option_rel,\<langle>nat_rel\<rangle>option_rel\<rangle>pairing_heaps_rel\<close> \<open>(i,j)\<in>nat_rel\<close>
+  shows \<open>mop_merge_pairs_imp xs i \<le> \<Down>(\<langle>\<langle>nat_rel\<rangle>option_rel,\<langle>nat_rel\<rangle>option_rel\<rangle>pairing_heaps_rel) (merge_pairs ys j)\<close>
+  using assms unfolding mop_merge_pairs_imp_def merge_pairs_def
+  by (refine_vcg mop_vsids_pass\<^sub>1_imp_spec mop_vsids_pass\<^sub>2_imp_spec) auto
+
+lemma vsids_pop_min_alt_def:
+  \<open>vsids_pop_min = (\<lambda>arr. do {
+  let h = source_node arr;
+  if h = None then RETURN (None, arr)
+  else do {
+      ASSERT (the h \<in> fst arr);
+      let j = hp_read_child' (the h) arr;
+      if j = None then RETURN (h, (update_source_node None arr))
+      else do {
+        ASSERT (the j \<in> fst arr);
+        let arr = hp_update_prev' (the h) None arr;
+        let arr = hp_update_child' (the h) None arr;
+        let arr = hp_update_parents' (the j) None arr;
+        arr \<leftarrow> merge_pairs (update_source_node None arr) (the j);
+        RETURN (h, arr)
+      }
+    }
+  })\<close> (is \<open>?A = ?B\<close>)
+proof -
+  have [simp]: \<open>source_node arr = None \<Longrightarrow> (fst arr, fst (snd arr), None) = arr\<close> for arr
+    by (cases arr) auto
+  have K[refine]: \<open>((source_node arr, fst arr, fst (snd arr), None), source_node arr,
+  update_source_node None arr)
+    \<in> Id\<close>
+    \<open>((source_node arr, update_source_node None arr), source_node arr, fst arr, fst (snd arr), None)
+    \<in> Id\<close>
+    for i arr
+    by (solves \<open>cases arr; auto\<close>)+
+  have [refine]: \<open>merge_pairs
+  (fst arr,
+   hp_update_parents (the (hp_read_child (the (source_node arr)) (fst (snd arr))))
+    None
+    (hp_update_child (the (source_node arr)) None
+      (hp_update_prev (the (source_node arr)) None (fst (snd arr)))),
+   None)
+  (the (hp_read_child (the (source_node arr)) (fst (snd arr))))
+    \<le> \<Down> Id
+    (merge_pairs
+      (update_source_node None
+     (hp_update_parents' (the (hp_read_child' (the (source_node arr)) arr)) None
+       (hp_update_child' (the (source_node arr)) None
+      (hp_update_prev' (the (source_node arr)) None arr))))
+    (the (hp_read_child' (the (source_node arr)) arr)))\<close>
+    \<open>merge_pairs
+   (update_source_node None
+  (hp_update_parents' (the (hp_read_child' (the (source_node arr)) arr)) None
+    (hp_update_child' (the (source_node arr)) None
+      (hp_update_prev' (the (source_node arr)) None arr))))
+   (the (hp_read_child' (the (source_node arr)) arr))
+  \<le> \<Down> Id
+  (merge_pairs
+    (fst arr,
+     hp_update_parents (the (hp_read_child (the (source_node arr)) (fst (snd arr)))) None
+      (hp_update_child (the (source_node arr)) None
+     (hp_update_prev (the (source_node arr)) None (fst (snd arr)))),
+     None)
+    (the (hp_read_child (the (source_node arr)) (fst (snd arr)))))\<close> for arr
+    by (solves \<open>cases arr; auto\<close>)+
+  have K: \<open>snd (snd arr) = source_node arr\<close> for arr
+    by (cases arr) auto
+
+  have \<open>?A arr \<le> \<Down>Id (?B arr)\<close> for i arr
+    unfolding vsids_pop_min_def case_prod_beta[of _ arr] case_prod_beta[of _ \<open>snd arr\<close>]
+      K
+    by refine_vcg (solves auto)+
+  moreover have \<open>?B arr \<le> \<Down>Id (?A arr)\<close> for i arr
+    unfolding vsids_pop_min_def case_prod_beta[of _ arr] case_prod_beta[of _ \<open>snd arr\<close>] K
+    by refine_vcg (solves \<open>auto intro!: ext bind_cong[OF refl] simp: Let_def\<close>)+
+  ultimately show ?thesis unfolding Down_id_eq apply -
+    apply (intro ext)
+    apply (rule antisym)
+    apply assumption+
+    done
+qed
+
+(*next*)
+
+thm vsids_pop_min_def
+  (*requires making a proper function out of it first for rescaling*)
+thm encoded_hp_prop_list_remove_find encoded_hp_prop_list_update_score
 end
